Veritas.MultiSet.fsti
@@ -50,6 +50,9 @@ let smap (#a:eqtype) (s1 s2: seq a) = f: (seq_index s1 -> seq_index s2)
 let into_smap (#a:eqtype) (s1 s2: seq a)  = f: smap s1 s2
   { forall (i: seq_index s1). forall (j: seq_index s1). (i <> j) ==> f i <> f j }
 
+val lemma_length_size (#a:eqtype) (s: seq a):
+  Lemma (length s = size (seq2mset s))
+
 (* if I provide a bijection between elements of two sequences that preserves equality,
  * the multisets of the two sequences should be the same *)
 val lemma_mset_bijection (#a:eqtype) (s1 s2: seq a) (f12: into_smap s1 s2) (f21: into_smap s2 s1):
